eliminate all sorry's of Network (#15)
* fix

* eliminate all sorry's!

LeanYjs/Network/OperationNetwork.lean
@@ -4,15 +4,15 @@ open NetworkModels
 
 variable {A I : Type}  [DecidableEq A] [Operation A] [DecidableEq I] [Message A I]
 
-def interpOps (items : List A) : Except (Operation.Error A) (Operation.State A) :=
-  List.foldlM (init := Operation.init) (f := fun acc item => Operation.effect item acc) items
+def interpOps (items : List A) (init : Operation.State A) : Except (Operation.Error A) (Operation.State A) :=
+  List.foldlM (init := init) (f := fun acc item => Operation.effect item acc) items
 
-def interpHistory (history : List (Event A)) : Except (Operation.Error A) (Operation.State A) :=
-  interpOps (history.filterMap (fun ev => match ev with | Event.Deliver it => some it | _ => none))
+def interpHistory (history : List (Event A)) (init : Operation.State A) : Except (Operation.Error A) (Operation.State A) :=
+  interpOps (history.filterMap (fun ev => match ev with | Event.Deliver it => some it | _ => none)) init
 
-def interpDeliveredOps {network : CausalNetwork A} (items : List (CausalNetworkElem A network)) : Except (Operation.Error A) (Operation.State A) :=
+def interpDeliveredOps {network : CausalNetwork A} (items : List (CausalNetworkElem A network)) (init : Operation.State A) : Except (Operation.Error A) (Operation.State A) :=
   let deliveredItems := items.map (fun item => item.elem)
-  interpOps deliveredItems
+  interpOps deliveredItems init
 
 class ValidMessage A [Operation A] where
   isValidMessage : Operation.State A → A → Prop
@@ -21,5 +21,5 @@ structure OperationNetwork A {I} [DecidableEq A] [DecidableEq I] [Operation A] [
   broadcast_only_valid_messages :
     ∀i, pre ++ [Event.Broadcast e] ++ post = histories i →
     ∃state,
-      interpHistory pre = Except.ok state ∧
-      ∀ {e i}, Event.Broadcast e ∈ histories i → ValidMessage.isValidMessage state e
+      interpHistory pre Operation.init = Except.ok state ∧
+      ValidMessage.isValidMessage state e
